Make various definitions opaque to improve verification performance

src/crypto/aes/GHash_s.fst
@@ -1,5 +1,6 @@
 module GHash_s
 
+open Opaque_s
 open Words_s
 open Types_s
 open GF128_s
@@ -15,13 +16,14 @@ let gf128_mul_LE (a_LE b_LE:quad32) : quad32 =
   let ab_BE = gf128_to_quad32 (gf128_mul (gf128_of_quad32 a_BE) (gf128_of_quad32 b_BE)) in
   reverse_bytes_quad32 ab_BE
 
-let rec ghash_LE (h_LE:quad32) (x:ghash_plain_LE) : Tot quad32 (decreases %[length x]) = 
+let rec ghash_LE_def (h_LE:quad32) (x:ghash_plain_LE) : Tot quad32 (decreases %[length x]) = 
   let y_i_minus_1 =
     (if length x = 1 then
        Mkfour 0 0 0 0
      else
-       ghash_LE h_LE (all_but_last x)) in
+       ghash_LE_def h_LE (all_but_last x)) in
   let x_i = last x in
   let xor_LE = quad32_xor y_i_minus_1 x_i in
   gf128_mul_LE xor_LE h_LE
 
+let ghash_LE = make_opaque ghash_LE_def
