src/crypto/aes/GCM_s.fst
@@ -1,5 +1,6 @@
 module GCM_s
 
+open Opaque_s
 open Words_s
 open Words.Seq_s
 open Types_s
@@ -14,7 +15,7 @@ unfold type gcm_auth_LE = gctr_plain_LE
 
 #reset-options "--z3rlimit 30"
 // little-endian, except for iv_BE
-let gcm_encrypt_LE (alg:algorithm) (key:aes_key alg) (iv:seqn 16 nat8) (plain:seq nat8) (auth:seq nat8) :
+let gcm_encrypt_LE_def (alg:algorithm) (key:aes_key alg) (iv:seqn 16 nat8) (plain:seq nat8) (auth:seq nat8) :
   Pure (tuple2 (seq nat8) (seq nat8))
     (requires
       4096 * length plain < pow2_32 /\
@@ -26,20 +27,34 @@ let gcm_encrypt_LE (alg:algorithm) (key:aes_key alg) (iv:seqn 16 nat8) (plain:se
   let iv_BE = be_bytes_to_quad32 iv in
   let h_LE = aes_encrypt_LE alg key_LE (Mkfour 0 0 0 0) in
   let j0_BE = Mkfour 1 iv_BE.lo1 iv_BE.hi2 iv_BE.hi3 in
-  
+
   let c = gctr_encrypt_LE (inc32 j0_BE 1) plain alg key_LE in
-  
+
   let lengths_BE = Mkfour (8 * length plain) 0 (8 * length auth) 0 in
   let lengths_LE = reverse_bytes_quad32 lengths_BE in
-  
+
   let zero_padded_c_LE = le_bytes_to_seq_quad32 (pad_to_128_bits c) in
   let zero_padded_a_LE = le_bytes_to_seq_quad32 (pad_to_128_bits auth) in
-  
+
   let hash_input_LE = append zero_padded_a_LE (append zero_padded_c_LE (create 1 lengths_LE)) in
   let s_LE = ghash_LE h_LE hash_input_LE in
   let t = gctr_encrypt_LE j0_BE (le_quad32_to_bytes s_LE) alg key_LE in
 
   (c, t)
+
+//let gcm_encrypt_LE = make_opaque gcm_encrypt_LE_def
+//REVIEW: unexpectedly, the following fails:
+//  let fails () : Lemma (gcm_encrypt_LE == make_opaque gcm_encrypt_LE_def) = ()
+//So we do this instead:
+let gcm_encrypt_LE (alg:algorithm) (key:aes_key alg) (iv:seqn 16 nat8) (plain:seq nat8) (auth:seq nat8) :
+  Pure (tuple2 (seq nat8) (seq nat8))
+    (requires
+      4096 * length plain < pow2_32 /\
+      4096 * length auth < pow2_32
+    )
+    (ensures fun (c, t) -> True)
+  =
+  make_opaque (gcm_encrypt_LE_def alg key iv plain auth)
 
 let gcm_decrypt_LE (alg:algorithm) (key:aes_key alg) (iv:seqn 16 nat8) (cipher:seq nat8) (auth:seq nat8) (tag:seq nat8) :
   Pure (tuple2 (seq nat8) (bool))
